## Derivatives Rules
(f(x)*g(x))' = f'(x)*g(x) + f(x)*g'(x)
(f(g(x)))' = f'(g(x))*g'(x)
## Derivatives
(N)' = 1
(N^(1/2))' = 1/2*N^(1/2)
(N^(1.5))' = 3/2*N^(1/2)
(N^2)' = 2N
(NlnN)' = 1*lnN + N*(1/N) = lnN + 1
(NlnlnN)' = 1*lnlnN + N*(lnlnN)' = lnlnN + N*(1/lnN)*(1/N) = lnlnN + 1/lnN
(N(lnN)^2)' = 1*(lnN)^2 + N*((lnN)^2)' = (lnN)^2 + N*(2lnN)*(1/N) = (lnN)^2 + 2lnN
(Nln(N^2))' = (2NlnN)' = 2(NlnN)' = 2lnN + 2
(2/N)' = -2/N^2
(2^N)' = ln2*2^N
(2^(N/2))' = ln2*2^N*(1/2) = ln2*2^N / 2
(37)' = 0
(N^2*lnN)' = 2N*lnN + N^2*(1/N) = 2NlnN + N
(N^3)' = 3N^2
